user 10, session 10, part 29

diffs-annotated-with-times/10/user-10-session-10.v
@@ -6,13 +6,17 @@ Set Printing Depth 50.
 Remove Search Blacklist "Private_" "_subproof".
 Add Search Blacklist "Private_" "_subproof".
 From Coq Require Import Basics ExtrOcamlIntConv List NArith String.
+From ReductionEffect Require Import PrintingEffect.
+Redirect "/var/folders/lm/cpf87_lx21n9bgnl4kr72rjm0000gn/T/coqfwCzEG"
+Print Ltac Signatures.
+Timeout 1 Print Grammar tactic.
+Timeout 1 Print LoadPath.
 From ExtLib Require Import Applicative Functor Monad StateMonad.
 From ITree Require Import Exception ITree Nondeterminism.
 From SimpleIO Require Import IO_Random SimpleIO.
 From QuickChick Require Import Decidability Show.
 From DeepWeb Require Import Exp.
-Import ApplicativeNotation FunctorNotation ListNotations MonadNotation
-SumNotations.
+Import ApplicativeNotation FunctorNotation ListNotations MonadNotation SumNotations.
 Open Scope N_scope.
 Open Scope monad_scope.
 Open Scope program_scope.
@@ -26,11 +30,10 @@ Definition derive_public (k : secret_key) : public_key := base ^ k mod prime.
 Definition calculate_shared (s : secret_key) (p : public_key) : shared_key :=
   p ^ s mod prime.
 Definition cipher_text := prod shared_key.
-Definition cipher {plain_text} :
-  shared_key -> plain_text -> cipher_text plain_text := pair.
-Definition decipher {plain_text} (s : shared_key)
-  (c : cipher_text plain_text) : option plain_text :=
-  let (k, t) := c in if s =? k then Some t else None.
+Definition cipher {plain_text} : shared_key -> plain_text -> cipher_text plain_text :=
+  pair.
+Definition decipher {plain_text} (s : shared_key) (c : cipher_text plain_text) :
+  option plain_text := let (k, t) := c in if s =? k then Some t else None.
 Definition random := N.
 Anomaly ""Assert_failure printing/ppconstr.ml:399:14"."
 Please report at http://coq.inria.fr/bugs/.
@@ -45,8 +48,7 @@ Instance showData : (Show (kvs_data id)) :=
          match d with
          | Kvs_GET k => "GET " ++ show k
          | Kvs_PUT k v => "PUT " ++ show k ++ " " ++ show v
-         | Kvs_CAS k x v =>
-             "CAS " ++ show k ++ " " ++ show x ++ " " ++ show v
+         | Kvs_CAS k x v => "CAS " ++ show k ++ " " ++ show x ++ " " ++ show v
          | Kvs_OK v => "OK  " ++ show (v : N)
          | Kvs_NoContent => "204"
          | Kvs_BadRequest => "400"
@@ -58,8 +60,7 @@ Instance showDataX : (Show (kvs_data exp)) :=
          match d with
          | Kvs_GET k => "GET " ++ show k
          | Kvs_PUT k v => "PUT " ++ show k ++ " " ++ show v
-         | Kvs_CAS k x v =>
-             "CAS " ++ show k ++ " " ++ show x ++ " " ++ show v
+         | Kvs_CAS k x v => "CAS " ++ show k ++ " " ++ show x ++ " " ++ show v
          | Kvs_OK v => "OK  " ++ show v
          | Kvs_NoContent => "204"
          | Kvs_BadRequest => "400"
@@ -93,29 +94,22 @@ Definition kvs : itree smE void :=
          match kvs_get k st with
          | Some v => embed App_Send (Kvs_OK v);; call st
          | None =>
-             v <- trigger Eval_Var;;
-             embed App_Send (Kvs_OK v);; call (kvs_put k v st)
+             v <- trigger Eval_Var;; embed App_Send (Kvs_OK v);; call (kvs_put k v st)
          end
-     | Kvs_PUT k v =>
-         embed App_Send Kvs_NoContent;; call (kvs_put k (exp_int v) st)
+     | Kvs_PUT k v => embed App_Send Kvs_NoContent;; call (kvs_put k (exp_int v) st)
      | Kvs_CAS k x v' =>
          match kvs_get k st with
          | Some v =>
              b <- trigger (Eval_Decide (exp_eq x v));;
              (if b : bool
-              then
-               embed App_Send Kvs_NoContent;;
-               call (kvs_put k (exp_int v') st)
+              then embed App_Send Kvs_NoContent;; call (kvs_put k (exp_int v') st)
               else embed App_Send Kvs_PreconditionFailed;; call st)
          | None =>
              v <- trigger Eval_Var;;
              b <- trigger (Eval_Decide (exp_eq x v));;
              (if b : bool
-              then
-               embed App_Send Kvs_NoContent;;
-               call (kvs_put k (exp_int v') st)
-              else
-               embed App_Send Kvs_PreconditionFailed;; call (kvs_put k v st))
+              then embed App_Send Kvs_NoContent;; call (kvs_put k (exp_int v') st)
+              else embed App_Send Kvs_PreconditionFailed;; call (kvs_put k v st))
          end
      | _ => embed App_Send Kvs_BadRequest;; call st
      end) [].
@@ -158,8 +152,7 @@ Instance showErr : (Show err) :=
          match e with
          | Err_Decide bx => "Cannot decide: " ++ show bx
          | Err_Guard rx r => "Guard error: " ++ show rx ++ " <> " ++ show r
-         | Err_Mismatch e0 te =>
-             "Events mismatch: " ++ show e0 ++ " <> " ++ show te
+         | Err_Mismatch e0 te => "Events mismatch: " ++ show e0 ++ " <> " ++ show te
          | Err_Unify bx b => "Cannot unify: " ++ show bx ++ " <> " ++ show b
          end |}.
 Definition nmi_of_smi {T} (m : itree smE T) :
@@ -178,10 +171,6 @@ Definition nmi_of_smi {T} (m : itree smE T) :
              end
          end
      end) m.
-Redirect "/var/folders/lm/cpf87_lx21n9bgnl4kr72rjm0000gn/T/coqLMjfun"
-Print Ltac Signatures.
-Timeout 1 Print Grammar tactic.
-Timeout 1 Print LoadPath.
 Anomaly ""Assert_failure printing/ppconstr.ml:399:14"."
 Please report at http://coq.inria.fr/bugs/.
 Definition unifier_of_smi :
@@ -195,28 +184,24 @@ Definition unifier_of_smi :
          match sae in (appE _ Y) return ((Y -> _) -> _) with
          | App_Recv =>
              fun k =>
-             r <- trigger Random_Request;;
-             embed App_Send r;; unifier_of_smi_rec (k r)
+             r <- trigger Random_Request;; embed App_Send r;; unifier_of_smi_rec (k r)
          | App_Send rx =>
              fun k =>
-             r <- embed App_Recv;;
-             trigger (Unify_Guard rx r);; unifier_of_smi_rec (k tt)
+             r <- embed App_Recv;; trigger (Unify_Guard rx r);; unifier_of_smi_rec (k tt)
          end k
      | VisF (|ee) k =>
          match ee in (evalE Y) return ((Y -> _) -> _) with
          | Eval_Var => bind (trigger Unify_New) \226\136\152 compose unifier_of_smi_rec
-         | Eval_Decide bx =>
-             bind (embed Unify_Decide bx) \226\136\152 compose unifier_of_smi_rec
+         | Eval_Decide bx => bind (embed Unify_Decide bx) \226\136\152 compose unifier_of_smi_rec
          end k
      end.
 Notation taE := (appE id +' exceptE err +' nondetE +' randomE).
 Anomaly ""Assert_failure printing/ppconstr.ml:399:14"."
 Please report at http://coq.inria.fr/bugs/.
-Definition liftState {s a : Type} {m : Type -> Type} 
-  `{Functor m} : m a -> stateT s m a :=
-  @mkStateT s m a \226\136\152 flip compose (flip pair) \226\136\152 flip fmap.
-Definition tester_of_unifier (u : itree (appE id +' unifyE +' randomE) unit)
-  : stateT state (itree taE) unit :=
+Definition liftState {s a : Type} {m : Type -> Type} `{Functor m} :
+  m a -> stateT s m a := @mkStateT s m a \226\136\152 flip compose (flip pair) \226\136\152 flip fmap.
+Definition tester_of_unifier (u : itree (appE id +' unifyE +' randomE) unit) :
+  stateT state (itree taE) unit :=
   interp
     (fun X e =>
      match e with
@@ -224,5 +209,155 @@ Definition tester_of_unifier (u : itree (appE id +' unifyE +' randomE) unit)
      | (e|) | (||e) => @liftState state X (itree taE) _ (trigger e)
      end) u.
 End App.
-(* Auto-generated comment: Succeeded. *)
+Module Network.
+Anomaly ""Assert_failure printing/ppconstr.ml:399:14"."
+Please report at http://coq.inria.fr/bugs/.
+Instance showPlainMessage : (Show plain_message) :=
+ {|
+ show := fun pm =>
+         match pm with
+         | PlainMessage_Hello messageRandom messagePublic =>
+             "Hello! random: " ++
+             show messageRandom ++ ", public key: " ++ show messagePublic
+         | PlainMessage_Finished verifyData =>
+             "Finished! verify data: " ++ show verifyData
+         | PlainMessage_AppData kvsData => "Application Data! " ++ show kvsData
+         | PlainMessage_BadRequest => "Bad Request!"
+         end |}.
+Inductive message :=
+  | Message_Plain : forall plainMessage : plain_message, _
+  | Message_Cipher : forall cipherMessage : cipher_text plain_message, _.
+Derive Show for message.
+Instance eqMessage  (x y : message): (Dec (x = y)).
+Proof.
+dec_eq.
+Defined.
+Definition Message_Finished (k : shared_key) (verifyData : N) : message :=
+  Message_Cipher (cipher k (PlainMessage_Finished verifyData)).
+Definition Message_Hello (messageRandom : random) (messagePublic : public_key) :
+  message := Message_Plain (PlainMessage_Hello messageRandom messagePublic).
+Anomaly ""Assert_failure printing/ppconstr.ml:399:14"."
+Please report at http://coq.inria.fr/bugs/.
+Anomaly ""Assert_failure printing/ppconstr.ml:399:14"."
+Please report at http://coq.inria.fr/bugs/.
+Import App.
+Anomaly ""Assert_failure printing/ppconstr.ml:399:14"."
+Please report at http://coq.inria.fr/bugs/.
+Derive Show for error.
+Notation hsE := (networkE +' exceptE error +' hsgenE).
+Anomaly ""Assert_failure printing/ppconstr.ml:399:14"."
+Please report at http://coq.inria.fr/bugs/.
+Anomaly ""Assert_failure printing/ppconstr.ml:399:14"."
+Please report at http://coq.inria.fr/bugs/.
+Definition map_exceptE {e1} {e2} (f : e1 -> e2) : exceptE e1 ~> exceptE e2 :=
+  fun _ e => match e with
+             | Throw e => Throw (f e)
+             end.
+Definition network_of_app {nE} `{networkE -< nE} `{exceptE error -< nE} 
+  {E} `{E -< nE} (k : shared_key) T (e : (appE id +' exceptE err +' E) T) : 
+  itree nE T :=
+  match e with
+  | (ae|) =>
+      match ae with
+      | App_Recv =>
+          msg <- trigger Network_Recv;;
+          match msg with
+          | Message_Plain _ => throw Error_UnexpectedMessage
+          | Message_Cipher msg =>
+              match decipher k msg with
+              | Some msg =>
+                  match msg with
+                  | PlainMessage_AppData data => ret data
+                  | _ => throw Error_UnexpectedMessage
+                  end
+              | None => throw Error_UnexpectedMessage
+              end
+          end
+      | App_Send data =>
+          embed Network_Send (Message_Cipher (cipher k (PlainMessage_AppData data)))
+      end
+  | (|(ee|)) => trigger (map_exceptE Error_App _ ee)
+  | (||e) => trigger e
+  end.
+Notation sE := (networkE +' exceptE error +' hsgenE +' randomE).
+Notation tE := (nondetE +' sE).
+CoFixpoint match_event {X} (e0 : networkE X) (x0 : X) (t : itree tE unit) : 
+itree tE unit :=
+  match t.(observe) with
+  | RetF r => Ret r
+  | TauF t => Tau (match_event e0 x0 t)
+  | VisF e k =>
+      match e with
+      | (|(ne|)) =>
+          match e0 in (networkE X), ne in (networkE Y) return ((Y -> _) -> X -> _) with
+          | Network_Recv, Network_Recv => id
+          | Network_Send m1, Network_Send m2 =>
+              if m1 = m2 ? then id else fun _ _ => throw Error_UnexpectedMessage
+          | _, _ => fun _ _ => throw Error_UnexpectedBehavior
+          end k x0
+      | (e|) | (||e|) | (|||e|) | (||||e) => vis e (match_event e0 x0 \226\136\152 k)
+      end
+  end.
+Definition match_event_list {X} :
+  networkE X -> X -> list (itree tE unit) -> list (itree tE unit) :=
+  compose pfmap \226\136\152 match_event.
+Definition server : itree sE void :=
+  sk <- translate subevent serverHandshake;; interp (network_of_app sk) (nmi_of_smi kvs).
+Anomaly ""Assert_failure printing/ppconstr.ml:399:14"."
+Please report at http://coq.inria.fr/bugs/.
+Anomaly ""Assert_failure printing/ppconstr.ml:399:14"."
+Please report at http://coq.inria.fr/bugs/.
+Definition showSE (se : sigT (fun X => sE X * X)%type) : string :=
+  match se with
+  | existT _ _ er =>
+      let (e, r) := er in
+      match e with
+      | (ne|) =>
+          match ne in (networkE X) return (X -> _) with
+          | Network_Recv => fun m => "Recv            : " ++ show m
+          | Network_Send m => fun _ => "Send            : " ++ show m
+          end r
+      | (|(Throw _|)) => "This message should never be printed."
+      | (||hge|) =>
+          match hge in (hsgenE X) return (X -> _) with
+          | HsGen_Key => fun k => "Generate Key    : " ++ show k
+          | HsGen_Random => fun r => "Generate Random : " ++ show r
+          end r
+      | (|||re) =>
+          match re in (randomE X) return (X -> _) with
+          | Random_Value => fun n => "Generate Value  : " ++ show n
+          | Random_Requst => fun r => "Generate Request: " ++ show r
+          end r
+      end
+  end.
+Definition showTE (te : sigT (fun X => tE X * X)%type) : string :=
+  match te with
+  | existT _ _ er =>
+      let (e, r) := er in
+      match e with
+      | (ne|) =>
+          match ne in (nondetE X) return (X -> _) with
+          | Or => fun b => "Flip coin       : " ++ show b
+          end r
+      | (|se) => showSE (existT _ _ (se, r))
+      end
+  end.
+Instance showEvent : (Show event) :=
+ {|
+ show := fun e =>
+         match e with
+         | Event_Tester te => "Tester " ++ showTE te
+         | Event_Server se => "Server " ++ showSE se
+         | Event_Retry e => "Retry upon exception   : " ++ show e
+         end |}.
+Anomaly ""Assert_failure printing/ppconstr.ml:399:14"."
+Please report at http://coq.inria.fr/bugs/.
+Notation zE := (exceptE error +' traceE +' hsgenE +' randomE +' nondetE).
+Redirect "/var/folders/lm/cpf87_lx21n9bgnl4kr72rjm0000gn/T/coqtcCzhj"
+Print Ltac Signatures.
+Timeout 1 Print Grammar tactic.
+Timeout 1 Print LoadPath.
+Anomaly ""Assert_failure printing/ppconstr.ml:399:14"."
+Please report at http://coq.inria.fr/bugs/.
+(* Auto-generated comment: Failed. *)
 
